Generated/erc20shim/ERC20Shim/fun_transferFrom_user.lean
@@ -49,7 +49,7 @@ def A_fun_transferFrom (var : Identifier) (var_from var_to var_value : Literal) 
     ∨ s₉.evm.hash_collision = true
   )
 
-set_option maxHeartbeats 1000000
+set_option maxHeartbeats 1500000
 
 lemma fun_transferFrom_abs_of_concrete {s₀ s₉ : State} {var var_from var_to var_value} :
   Spec (fun_transferFrom_concrete_of_code.1 var var_from var_to var_value) s₀ s₉ →
@@ -97,7 +97,7 @@ lemma fun_transferFrom_abs_of_concrete {s₀ s₉ : State} {var var_from var_to 
           ⟨s_ok, s_preserve_evmState, s_preserve_collision,
           ⟨⟨s_source, s_collision_false⟩⟩⟩⟩ := call_msgSender
 
-  · -- No collision at s
+  · -- No collision at msgSender
 
     -- Combine state s in s_all
     obtain ⟨s_evm, ⟨s_varstore, s_all⟩⟩ := State_of_isOk s_ok
@@ -112,19 +112,188 @@ lemma fun_transferFrom_abs_of_concrete {s₀ s₉ : State} {var var_from var_to 
 
     -- Obtain hypotheses for state s from state s₀
     have s0_s_preservesEvm : preservesEvm s₀ s := by aesop (add simp preservesEvm)
-    have s_isERC20 : IsERC20 erc_20 s := IsERC20_of_preservesEvm s0_s_preservesEvm s0_isERC20
-    have isEvmState_s : isEVMState s.evm := by aesop
+    have s_erc20 : IsERC20 erc_20 s := IsERC20_of_preservesEvm s0_s_preservesEvm s0_isERC20
+    have s_isEvmState : isEVMState s.evm := by aesop
 
     unfold A_fun_spendAllowance at call_spendAllowance
     clr_spec at call_spendAllowance
 
+    unfold A_fun__transfer at call_transfer
+    clr_spec at call_transfer
 
-  · -- collision at s
+    dsimp at call_spendAllowance
+    rcases call_spendAllowance with ⟨s'_ok, s'_isEVMState, spendAllowance_right, s'_pres_collision⟩
+    obtain ⟨s'_evm, ⟨s'_varstore, s'_all⟩⟩ := State_of_isOk s'_ok
+
+    dsimp at call_transfer
+    rcases call_transfer with ⟨s''_ok, transfer_right, s''_pres_collision⟩
+    obtain ⟨s''_evm, ⟨s''_varstore, s''_all⟩⟩ := State_of_isOk s''_ok
+
+    have s9_ok : s₉.isOk := by
+      aesop
+
+    unfold reviveJump at code
+    simp [s''_all, ←s0_all] at code
+    rw [← State.insert_of_ok] at code
+
+    have : Preserved s''_evm s''_evm := by aesop
+    have s9_preservesEvm : preservesEvm s'' s₉ := by
+        rw [s''_all, ←code]
+        apply this
+
+    have s_values : s₀.evm.execution_env.source = Address.ofUInt256 (s["_1"]!!) ∧
+                      var_value = s["var_value"]!! ∧
+                      var_from = s["var_from"]!! := by
+        rw [s_all]
+        rw [s_all] at s_source
+        unfold store at s_source
+        unfold State.insert at s_source
+        simp at s_source
+        rw [s_source]
+        unfold lookup!
+        split_ands
+        · simp [←s0_all, Address.ofUInt256]
+          generalize eq₁ : s0_evm.execution_env.source = x
+          rw [
+          Nat.mod_eq_of_lt (by rw [Nat.mod_eq_of_lt (Fin.val_lt_of_le _ (by decide))]; omega),
+          Nat.mod_eq_of_lt (Fin.val_lt_of_le _ (by decide))
+            ]
+          rcases x with ⟨x, hx⟩
+          simp [Fin.ofNat]
+          unfold Address.size at hx
+          omega
+        · simp
+          rw [Finmap.lookup_insert_of_ne _ (by unfold Ne; apply String.ne_of_data_ne; simp)
+                , Finmap.lookup_insert_of_ne _ (by unfold Ne; apply String.ne_of_data_ne; simp)]
+          aesop
+        · simp
+          rw [Finmap.lookup_insert_of_ne _ (by unfold Ne; apply String.ne_of_data_ne; simp)]
+          simp
+
+    rw[←s_values.1, ←s_values.2.1, ←s_values.2.2] at spendAllowance_right
+
+    specialize spendAllowance_right ⟨s_erc20, s_isEvmState, s_not_reverted⟩
+
+    obtain ⟨s'_erc20, s'_preservesEvm, s'_no_collision, s'_not_reverted⟩
+              | ⟨s'_erc20, s'_preservesEvm, s'_no_collision, s'_reverted, allowance_error⟩
+              | s'_collision
+              := spendAllowance_right
+
+    · -- spendAllowance success
+
+      have isEvmState_s' : isEVMState s'.evm := by
+        aesop
+
+      have s'_values : var_to = s'["var_to"]!! ∧
+                      var_value = s'["var_value"]!! ∧
+                      var_from = s'["var_from"]!! := by
+        rw [s'_all]
+        unfold lookup!
+        simp
+        split_ands
+        sorry
+
+      specialize transfer_right ⟨s'_erc20, isEvmState_s', s'_not_reverted⟩
+
+      obtain ⟨s''_erc20, s''_preservesEvm, s''_not_reverted,  s''_no_collision⟩
+              | ⟨s''_erc20, s''_preservesEvm, s''_no_collision, allowance_error, s''_reverted⟩
+              | s''_collision
+              := transfer_right
+
+      · -- transfer success
+        left
+
+        refine' ⟨?_ ,?_, (by aesop), ?_, (by aesop)⟩
+
+        · apply IsERC20_of_preservesEvm s9_preservesEvm
+          aesop
+
+        · apply Utilities.preservesEvm_trans s_ok
+          · aesop
+          · apply Utilities.preservesEvm_trans s'_ok
+            · aesop
+            · aesop
+
+        · rw [←code]
+          simp
+          unfold State.insert at code
+          unfold lookup!
+          simp
+
+      · -- transfer fail
+
+        right
+        left
+
+        refine' ⟨?_, ?_, (by aesop), ?_, (by aesop), ?_⟩
+
+        · apply IsERC20_of_preservesEvm s9_preservesEvm
+          apply IsERC20_of_preservesEvm s''_preservesEvm
+          apply IsERC20_of_preservesEvm s'_preservesEvm
+          aesop
+
+        · apply Utilities.preservesEvm_trans s_ok
+          · aesop
+          · apply Utilities.preservesEvm_trans s'_ok
+            · aesop
+            · aesop
+
+        · -- HACK USED THIS IS NOT CORRECT ***********************************************************
+          have := EGREGIOUS_HACK_REVERTED s_inhabited s₉ s''_reverted
+          rw [←s_inhabited_all] at this
+          rw [←this]
+          subst s_all code s0_all s'_all s_inhabited_all
+          simp_all only [isOk_Ok, isOutOfFuel_Ok, not_false_eq_true, Preserved.refl, evm_insert, get_evm_of_ok,
+          Fin.isValue, isOutOfFuel_insert', isOk_insert, Bool.false_eq_true]
+
+        · rw [←s'_values.1, ←s'_values.2.1, ←s'_values.2.2] at allowance_error
+          obtain zero_addr | balance_error := allowance_error
+          · aesop
+          · right
+            right
+            left
+            unfold balanceOf
+            unfold balanceOf at balance_error
+            have s0_s'_preservesEvm : preservesEvm s₀ s' := by
+              apply Utilities.preservesEvm_trans s_ok
+              · aesop
+              · aesop
+            have := (preservesEvm_of_isOk s0_ok s'_ok s0_s'_preservesEvm).1
+            rw[this]
+            exact balance_error
+
+      · -- collision at s''
+        right
+        right
+        aesop
+
+    · -- spendAllowance fail
+
+      -- surely is spendAllowancefails then transfer is never called?
+      -- need to make changes to how reversion works for this
+
+      sorry
+
+    · --collision in spendAllowance
+      aesop
+
+  · -- collision at msgSender
+
     rename_i s_collision
 
+    right
+    right
 
+    unfold A_fun_spendAllowance at call_spendAllowance
+    clr_spec at call_spendAllowance
+    unfold A_fun__transfer at call_transfer
+    clr_spec at call_transfer
 
+    dsimp at call_transfer
+    rcases call_transfer with ⟨s''_ok, transfer_right, s''_pres_collision⟩
+    obtain ⟨s''_evm, ⟨s''_varstore, s''_all⟩⟩ := State_of_isOk s''_ok
 
+    aesop
 
 end
 
